finish simple exercises

software-foundations/programming-language-foundations/HoareLogic/Examples.v
@@ -204,3 +204,282 @@ Proof.
     now apply parity_lt_2.
   - intros st H. auto.
 Qed.
+
+Definition factorial : com :=
+  (* X = m *)
+  Y ::= 1 ;;
+  (* Y * X! = m! *)
+  WHILE ¬ (X = 0) DO
+    (* Y * X! = m! ∧ X ≠ 0 *)
+    (* Y * X * (X - 1)! = m! *)
+    Y ::= Y * X ;;
+    (* Y * (X - 1)! = m! *)
+    X ::= X - 1
+    (* Y * X! = m! *)
+  END
+  (* Y * X! = m! ∧ ¬ (X ≠ 0) *)
+  (* Y = m! *)
+.
+
+Lemma negb_sym' : ∀ a b,
+  negb a = b → a = negb b.
+Proof.
+  intros. rewrite <- H.
+  now rewrite negb_involutive.
+Qed.
+
+Lemma fact_nz : ∀ x,
+  x ≠ 0 → fact x = x * fact (x - 1).
+Proof.
+  induction x.
+  - intros. contradiction.
+  - intros. simpl. now rewrite sub_0_r.
+Qed.
+
+Example factorial_proof : ∀ m,
+  {{ fun st => st X = m }}
+    factorial
+  {{ fun st => st Y = fact m }}.
+Proof.
+  unfold factorial. intros m.
+  apply hoare_seq with
+    (fun st => st Y * fact (st X) = fact m).
+  (* while *)
+  eapply hoare_consequence_post.
+  apply hoare_while.
+
+  (* while body *)
+  eapply hoare_seq.
+  (* X ::= X - 1 *)
+  apply hoare_assign.
+  (* Y ::= Y * X *)
+  eapply hoare_consequence_pre.
+  apply hoare_assign.
+
+  (* Y * X! = m! ∧ X ≠ 0 ->> Y * X * (X - 1)! = m! *)
+  - unfold assn_sub. unfold t_update. unfold bassn. simpl.
+    intros st [Y_X'_m' n_X_0].
+    apply negb_sym' in n_X_0.
+    apply beq_nat_false in n_X_0.
+    rewrite <- mult_assoc.
+    now rewrite <- (fact_nz (st X) n_X_0).
+
+  (* Y * X! = m! ∧ ¬ (X ≠ 0) ->> Y! = m! *)
+  - unfold bassn. simpl.
+    intros st [Y_X'_m' X_0].
+    apply not_true_is_false in X_0.
+    apply negb_sym' in X_0.
+    apply beq_nat_true in X_0.
+    rewrite X_0 in Y_X'_m'. simpl in Y_X'_m'.
+    now rewrite mult_1_r in Y_X'_m'.
+
+  (* Y ::= 1 *)
+  - eapply hoare_consequence_pre.
+    apply hoare_assign.
+    intros st Xm.
+    unfold assn_sub. unfold t_update. simpl.
+    rewrite plus_0_r. auto.
+Qed.
+
+Lemma min_0 : ∀ x y,
+  x = 0 ∨ y = 0 → min x y = 0.
+Proof.
+  intros. destruct H; rewrite H.
+  - apply min_0_l.
+  - apply min_0_r.
+Qed.
+
+Lemma min_minus_1 : ∀ x y,
+  min (x - 1) (y - 1) = min x y - 1.
+Proof.
+  destruct x; intros.
+  - simpl. reflexivity.
+  - destruct y; simpl.
+    + now rewrite min_0_r.
+    + now repeat rewrite sub_0_r.
+Qed.
+
+Definition imp_min : com :=
+  (* X = a ∧ Y = b *)
+  (* 0 + min X Y = min a b *)
+  Z ::= 0;;
+  (* Z + min X Y = min a b *)
+  WHILE (¬ (X = 0)) && (¬ (Y = 0)) DO
+    (* Z + min X Y = min a b ∧ (X ≠ 0) && (Y ≠ 0) *)
+    (* Z + 1 + min (X - 1) (Y - 1) = min a b *)
+    X ::= X - 1;;
+    (* Z + 1 + min X (Y - 1) = min a b *)
+    Y ::= Y - 1;;
+    (* Z + 1 + min X Y = min a b *)
+    Z ::= Z + 1
+    (* Z + min X Y = min a b *)
+  END
+  (* Z + min X Y = min a b ∧ ¬ ((X ≠ 0) && (Y ≠ 0))*)
+  (* Z = min a b *)
+.
+
+Lemma not_0_S : ∀ x,
+  x ≠ 0 → ∃ y, x = S y.
+Proof.
+  intros. destruct x.
+  - contradiction.
+  - now exists x.
+Qed.
+
+Lemma n_beq_nat_false : ∀ x y,
+  negb (x =? y) = false → x = y.
+Proof.
+  intros.
+  apply negb_sym' in H.
+  now apply beq_nat_true.
+Qed.
+
+Example imp_min_proof : ∀ a b,
+  {{ fun st => st X = a ∧ st Y = b }}
+    imp_min
+  {{ fun st => st Z = min a b }}.
+Proof.
+  unfold imp_min. intros a b.
+  apply hoare_seq with
+    (fun st => st Z + min (st X) (st Y) = min a b).
+
+  (* WHILE *)
+  eapply hoare_consequence_post.
+  (* WHILE body *)
+  apply hoare_while.
+  eapply hoare_seq.
+  eapply hoare_seq.
+  (* Z ::= Z + 1 *)
+  apply hoare_assign.
+  (* Y ::= Y - 1 *)
+  apply hoare_assign.
+  (* X ::= X - 1 *)
+  eapply hoare_consequence_pre.
+  apply hoare_assign.
+
+  (* Z + min X Y = min a b ∧ (X ≠ 0) && (Y ≠ 0) *)
+  (* Z + 1 + min (X - 1) (Y - 1) = min a b *)
+  - unfold bassn. unfold assn_sub. unfold t_update. simpl.
+    intros st [Z_minXY_minab n_X_0_n_Y_0].
+    apply andb_true_iff in n_X_0_n_Y_0 as [n_X_0 n_Y_0].
+    apply negb_sym' in n_X_0. apply beq_nat_false in n_X_0.
+    apply negb_sym' in n_Y_0. apply beq_nat_false in n_Y_0.
+    apply not_0_S in n_X_0 as [x' Ex'].
+    apply not_0_S in n_Y_0 as [y' Ey'].
+    rewrite Ex', Ey'. rewrite Ex', Ey' in Z_minXY_minab.
+    simpl. repeat rewrite sub_0_r.
+    simpl in Z_minXY_minab.
+    now rewrite <- add_assoc.
+  
+  (* Z + min X Y = min a b ∧ ¬ ((X ≠ 0) && (Y ≠ 0))*)
+  (* Z = min a b *)
+  - unfold bassn. simpl.
+    intros st [Z_minXY_minab n_X_0_Y_0].
+    apply not_true_is_false in n_X_0_Y_0.
+    apply andb_false_iff in n_X_0_Y_0 as [H | H];
+      apply n_beq_nat_false in H;
+      rewrite H in Z_minXY_minab;
+      [> rewrite min_0_l in Z_minXY_minab | rewrite min_0_r in Z_minXY_minab];
+      now rewrite plus_0_r in Z_minXY_minab.
+
+  (* Z ::= 0 *) 
+  - eapply hoare_consequence_pre.
+    apply hoare_assign.
+
+    (* X = a ∧ Y = b *)
+    (* 0 + min X Y = min a b *)
+    intros st [Xa Yb].
+    unfold assn_sub. unfold t_update. simpl.
+    congruence.
+Qed.
+
+(* two loops *)
+(*
+{{ True }}
+{{ 0 = 0 ∧ 0 = 0 ∧ c = 0 }}
+X ::= 0 ;;
+{{ X = 0 ∧ 0 = 0 ∧ c = 0 }}
+Y ::= 0 ;;
+{{ X = 0 ∧ Y = 0 ∧ c = 0 }}
+Z ::= c ;;
+{{ X = 0 ∧ Y = 0 ∧ Z = c }}
+{{ Z = X + c ∧ Y = 0 }}
+WHILE ¬ (X = a) DO
+  {{ Z = X + c ∧ Y = 0 ∧ X ≠ a }}
+  {{ Z + 1 = X + 1 + c }}
+  X ::= X + 1;;
+  {{ Z + 1 = X + c }}
+  Z ::= Z + 1
+  {{ Z = X + c ∧ Y = 0 }}
+END ;;
+{{ Z = X + c ∧ Y = 0 ∧ X = a }}
+{{ Z = Y + a + c }}
+WHILE ¬ (Y = b) DO
+  {{ Z = Y + a + c ∧ Y ≠ b }}
+  {{ Z + 1 = Y + 1 + a + c }}
+  Y ::= Y + 1;;
+  {{ Z + 1 = Y + a + c }}
+  Z ::= Z + 1
+  {{ Z = Y + a + c }}
+END
+{{ Z = Y + a + c ∧ Y = b }}
+{{ Z = a + b + c }}
+*)
+
+Lemma pow2_add : ∀ x,
+  2 ^ x + 2 ^ x = 2 ^ (x + 1).
+Proof.
+  induction x.
+  - reflexivity.
+  - simpl. repeat rewrite add_0_r.
+    now rewrite IHx.
+Qed.
+
+Example power_series : ∀ m : nat,
+  {{ fun st => st X = 0 ∧ st Y = 1 ∧ st Z = 1 }}
+    (* Y = 2 ^ (1 + X) - 1 ∧ Z = 2 ^ X *)
+    WHILE ¬ (X = m) DO
+      (* Y = 2 ^ (1 + X) - 1 ∧ Z = 2 ^ X ∧ X ≠ m *)
+      (* Y + 2 * Z = 2 ^ (1 + X + 1) - 1 ∧ 2 * Z = 2 ^ (X + 1)*)
+      Z ::= 2 * Z;;
+      (* Y + Z = 2 ^ (1 + X + 1) - 1 ∧ Z = 2 ^ (X + 1)*)
+      Y ::= Y + Z;;
+      (* Y = 2 ^ (1 + X + 1) - 1 ∧ Z = 2 ^ (X + 1)*)
+      X ::= X + 1
+      (* Y = 2 ^ (1 + X) - 1 ∧ Z = 2 ^ X *)
+    END
+    (* Y = 2 ^ (1 + X) - 1 ∧ Z = 2 ^ X ∧ X = m *)
+  {{ fun st => st Y = 2 ^ (1 + m) - 1 }}.
+Proof.
+  intros m.
+  apply hoare_consequence_pre with
+    (fun st => st Y = 2 ^ (1 + st X) - 1 ∧ st Z = 2 ^ st X).
+
+  all: cycle 1. (* solve the trivial one *)
+  (* X = 0 ∧ Y = 1 ∧ Z = 1 ->> Y = 2 ^ (1 + X) - 1 ∧ Z = 2 ^ X *)
+  intros st [X0 [Y1 Z1]]. rewrite X0, Y1, Z1. easy.
+
+  eapply hoare_consequence_post.
+  apply hoare_while.
+
+  all: cycle 1.
+  (* Y = 2 ^ (1 + X) - 1 ∧ Z = 2 ^ X ∧ X = m ->> Y = 2 ^ (1 + m) - 1 *)
+  unfold bassn. simpl. intros st [[Eyx Ezx] Xm].
+  apply not_true_is_false in Xm.
+  apply n_beq_nat_false in Xm.
+  congruence.
+
+  (* WHILE body *)
+  eapply hoare_seq.
+  eapply hoare_seq.
+  apply hoare_assign.
+  apply hoare_assign.
+  eapply hoare_consequence_pre.
+  apply hoare_assign.
+  unfold bassn. unfold assn_sub. unfold t_update. simpl.
+  intros st [[YX ZX] _]. rewrite YX, ZX. split.
+  - repeat rewrite add_0_r.
+    rewrite pow2_add. Omega.omega.
+  - rewrite add_0_r.
+    apply pow2_add.
+Qed.
